ISA/Bin.lean
@@ -1,0 +1,208 @@
+import Lean.LocalContext
+/-!
+
+- [opaque](https://lean-lang.org/doc/reference/latest/Definitions/Definitions/#Lean___Parser___Command___declaration-next-next-next-next-next-next-next-next-next-next-next)
+- [implemented_by](https://lean-lang.org/doc/reference/latest/Definitions/Recursive-Definitions/#Lean___Parser___Attr___simple)
+- [StateT](https://leanprover.github.io/functional_programming_in_lean/monad-transformers/transformers.html#state)
+- https://llvm.org/docs/LangRef.html#instruction-reference
+- https://en.wikipedia.org/wiki/X86#Structure
+- https://en.wikipedia.org/wiki/FLAGS_register
+- https://www.felixcloutier.com/x86/
+
+-/
+namespace X64
+
+opaque Byte : Type -- := UInt8
+structure Word where (highByte lowByte : Byte)
+structure Dword where (highWord lowWord : Word)
+structure Qword where (highDword lowDword : Dword)
+
+#check UInt16.toUInt8
+#check Lean.LocalDecl.isLet
+
+structure RegisterFile where
+  (rax rbx rcx rdx r8 r9 r10 r11 r12 r13 r14 r15 : Qword)
+  (cs ds ss es fs gs : Word)
+  (rsp rbp : Qword)
+  (rsi rdi : Qword)
+  (rip : Qword)
+  (cf pf af zf sf tf «if» df of iopl nt md rf vm ac vif vip id ai : Bool)
+
+namespace RegisterFile
+variable (self : RegisterFile)
+
+def eax : Dword := self.rax.lowDword
+def  ax :  Word := self.eax.lowWord
+def  ah :  Byte :=  self.ax.highByte
+def  al :  Byte :=  self.ax.lowByte
+
+def ebx : Dword := self.rbx.lowDword
+def  bx :  Word := self.ebx.lowWord
+def  bh :  Byte :=  self.bx.highByte
+def  bl :  Byte :=  self.bx.lowByte
+
+def ecx : Dword := self.rcx.lowDword
+def  cx :  Word := self.ecx.lowWord
+def  ch :  Byte :=  self.cx.highByte
+def  cl :  Byte :=  self.cx.lowByte
+
+def edx : Dword := self.rdx.lowDword
+def  dx :  Word := self.edx.lowWord
+def  dh :  Byte :=  self.dx.highByte
+def  dl :  Byte :=  self.dx.lowByte
+
+def r8d : Dword := self.r8.lowDword
+def r8w :  Word := self.r8d.lowWord
+def r8b :  Byte := self.r8w.lowByte
+
+def r9d : Dword := self.r9.lowDword
+def r9w :  Word := self.r9d.lowWord
+def r9b :  Byte := self.r9w.lowByte
+
+def r10d : Dword := self.r10.lowDword
+def r10w :  Word := self.r10d.lowWord
+def r10b :  Byte := self.r10w.lowByte
+
+def r11d : Dword := self.r11.lowDword
+def r11w :  Word := self.r11d.lowWord
+def r11b :  Byte := self.r11w.lowByte
+
+def r12d : Dword := self.r12.lowDword
+def r12w :  Word := self.r12d.lowWord
+def r12b :  Byte := self.r12w.lowByte
+
+def r13d : Dword := self.r13.lowDword
+def r13w :  Word := self.r13d.lowWord
+def r13b :  Byte := self.r13w.lowByte
+
+def r14d : Dword := self.r14.lowDword
+def r14w :  Word := self.r14d.lowWord
+def r14b :  Byte := self.r14w.lowByte
+
+def r15d : Dword := self.r15.lowDword
+def r15w :  Word := self.r15d.lowWord
+def r15b :  Byte := self.r15w.lowByte
+
+def esp : Dword := self.rsp.lowDword
+def  sp :  Word := self.esp.lowWord
+def  spl : Byte :=  self.sp.lowByte
+
+def ebp : Dword := self.rbp.lowDword
+def  bp :  Word := self.ebp.lowWord
+def  bpl : Byte :=  self.bp.lowByte
+
+def esi : Dword := self.rsi.lowDword
+def  si :  Word := self.esi.lowWord
+def  sil : Byte :=  self.si.lowByte
+
+def edi : Dword := self.rdi.lowDword
+def  di :  Word := self.edi.lowWord
+def  dil : Byte :=  self.di.lowByte
+
+def eip : Dword := self.rip.lowDword
+def  ip :  Word := self.eip.lowWord
+
+end RegisterFile
+
+def Byte.add : Byte → Byte → Byte × Bool := sorry
+def Word.add : Word → Word → Word × Bool := sorry
+def Dword.add : Dword → Dword → Dword × Bool := sorry
+def Qword.add : Qword → Qword → Qword × Bool := sorry
+
+def Byte.zeroExtendToWord : Byte → Word := sorry
+def Byte.signExtendToWord : Byte → Word × Bool := sorry
+def Byte.zeroExtendToDword : Byte → Dword := sorry
+def Byte.signExtendToDword : Byte → Dword × Bool := sorry
+def Byte.zeroExtendToQword : Byte → Qword := sorry
+def Byte.signExtendToQword : Byte → Qword × Bool := sorry
+
+def Word.zeroExtendToDword : Word → Dword := sorry
+def Word.signExtendToDword : Word → Dword × Bool := sorry
+def Word.zeroExtendToQword : Word → Qword := sorry
+def Word.signExtendToQword : Word → Qword × Bool := sorry
+
+def Dword.zeroExtendToQword : Dword → Qword := sorry
+def Dword.signExtendToQword : Dword → Qword × Bool := sorry
+
+inductive Qreg
+  | rax | rbx | rcx | rdx
+  -- | r8 | r9 | r10 | r11 | r12 | r13 | r14 | r15
+  -- | rsp | rbp
+  -- | rsi | rdi
+  -- | rip
+
+def addq {m} [Monad m] (rd rs1 rs2 : Qreg) : StateT RegisterFile m Unit := do
+  let regs ← get
+  let (sum, cf) := Qword.add (getReg regs rs1) (getReg regs rs2)
+  match rd with
+  | .rax => modify fun regs => {regs with rax := sum, cf}
+  | .rbx => modify fun regs => {regs with rbx := sum, cf}
+  | .rcx => modify fun regs => {regs with rcx := sum, cf}
+  | .rdx => modify fun regs => {regs with rdx := sum, cf}
+  where
+    getReg (regs : RegisterFile) : Qreg → Qword
+      | .rax => regs.rax
+      | .rbx => regs.rbx
+      | .rcx => regs.rcx
+      | .rdx => regs.rdx
+
+section
+
+inductive Bin'
+  | nil
+  | zed (b : Bin')
+  | one (b : Bin')
+
+inductive Bin
+  | nil
+  | pos (b : Bin')
+
+def Bin'.toNat : Bin' → Nat
+  | nil => 1
+  | zed b => 2 * b.toNat
+  | one b => 2 * b.toNat + 1
+
+def Bin.toNat : Bin → Nat
+  | nil => 0
+  | pos b => b.toNat
+
+def Bin'.succ : Bin' → Bin'
+  | nil => nil.zed
+  | zed b => b.one
+  | one b => b.succ.zed
+
+def Bin.succ : Bin → Bin
+  | nil => pos .nil
+  | pos b => pos b.succ
+
+def Bin.ofNat : Nat → Bin
+  | 0 => nil
+  | n + 1 => (ofNat n).succ
+
+
+theorem Bin.ofNat_of_toNat_eq_self : {b : Bin} → ofNat b.toNat = b
+  | nil => rfl
+  | pos b =>
+    calc ofNat b.toNat
+     _ = pos b := sorry
+
+theorem Bin'.toNat_of_succ_eq_succ_of_toNat : {b : Bin'} → b.succ.toNat = b.toNat + 1
+  | nil
+  | zed _ => rfl
+  | one b =>
+    show 2 * b.succ.toNat = 2 * (b.toNat + 1) from congrArg _ toNat_of_succ_eq_succ_of_toNat
+
+theorem Bin.toNat_of_succ_eq_succ_of_toNat : {b : Bin} → b.succ.toNat = b.toNat + 1
+  | nil => rfl
+  | pos b => show b.succ.toNat = b.toNat + 1 from b.toNat_of_succ_eq_succ_of_toNat
+
+theorem Bin.toNat_of_ofNat_eq_self : {n : Nat} → (ofNat n).toNat = n
+  | 0 => rfl
+  | n + 1 =>
+    calc (ofNat n).succ.toNat
+     _ = (ofNat n).toNat + 1 := toNat_of_succ_eq_succ_of_toNat
+     _ = n + 1 := congrArg _ toNat_of_ofNat_eq_self
+
+theorem Bin.ofNat_of_succ_eq_succ_of_ofNat : {n : Nat} → ofNat (n + 1) = (ofNat n).succ := rfl
+
+end
