Jacobson/Okasaki.lean
@@ -1,0 +1,60 @@
+set_option autoImplicit false
+
+/-- Binary Tree -/
+inductive BinTree α
+  | leaf
+  | node (data : α) (left right : BinTree α)
+
+abbrev RBTree α := BinTree (Bool × α)
+
+namespace BinTree
+variable {α}
+
+@[match_pattern]
+abbrev red (data : α) (left right : RBTree α) : RBTree α := node (false, data) left right
+
+@[match_pattern]
+abbrev black (data : α) (left right : RBTree α) : RBTree α := node (true, data) left right
+
+@[inline]
+def balanceLeft : α → RBTree α → RBTree α → RBTree α
+  | data₂, red data (red data₁ left₁ right₁) left₂, right₂
+  | data₂, red data₁ left₁ (red data right₁ left₂), right₂ =>
+    red data (black data₁ left₁ right₁) (black data₂ left₂ right₂)
+  | data, left, right => black data left right
+
+@[inline]
+def balanceRight : α → RBTree α → RBTree α → RBTree α
+  | data₁, left₁, red data₂ (red data right₁ left₂) right₂
+  | data₁, left₁, red data right₁ (red data₂ left₂ right₂) =>
+    red data (black data₁ left₁ right₁) (black data₂ left₂ right₂)
+  | data, left, right => black data left right
+
+end BinTree
+
+#check Decidable
+
+namespace BinTree
+variable {α}
+
+
+
+end BinTree
+
+class inductive Tree α {τ} : τ → Prop
+  | isLeaf {leaf} : Tree α leaf
+  | isNode {node left right : τ} (data : α) : Tree α left → Tree α right → Tree α node
+
+#check Subarray
+
+structure Heap α where
+  array : Array α
+  index : Nat
+
+instance Heap.tree {α} (heap : Heap α) : Tree α heap :=
+  if h : heap.index < heap.array.size then
+    .isNode heap.array[heap.index]
+      {heap with index := heap.index * 2 + 1}.tree
+      {heap with index := heap.index * 2 + 2}.tree
+  else
+    .isLeaf
